Prove tick-approximation for linked abstraction

doc/coq/.CoqMakefile.d
@@ -10,6 +10,9 @@ simple/Concrete.vos simple/Concrete.vok simple/Concrete.required_vos: simple/Con
 simple/Fixpoint.vo simple/Fixpoint.glob simple/Fixpoint.v.beautified simple/Fixpoint.required_vo: simple/Fixpoint.v simple/Abstract.vo
 simple/Fixpoint.vio: simple/Fixpoint.v simple/Abstract.vio
 simple/Fixpoint.vos simple/Fixpoint.vok simple/Fixpoint.required_vos: simple/Fixpoint.v simple/Abstract.vos
+simple/LinkSound.vo simple/LinkSound.glob simple/LinkSound.v.beautified simple/LinkSound.required_vo: simple/LinkSound.v simple/ALinking.vo simple/Linking.vo
+simple/LinkSound.vio: simple/LinkSound.v simple/ALinking.vio simple/Linking.vio
+simple/LinkSound.vos simple/LinkSound.vok simple/LinkSound.required_vos: simple/LinkSound.v simple/ALinking.vos simple/Linking.vos
 simple/Linking.vo simple/Linking.glob simple/Linking.v.beautified simple/Linking.required_vo: simple/Linking.v simple/Sound.vo
 simple/Linking.vio: simple/Linking.v simple/Sound.vio
 simple/Linking.vos simple/Linking.vok simple/Linking.required_vos: simple/Linking.v simple/Sound.vos
