doc/coq/simple/LinkSound.v
@@ -1,0 +1,326 @@
+From Simple Require Export ALinking.
+From Simple Require Export Linking.
+
+Module AL := ALinking.
+Module CL := Linking.
+
+Generalizable Variables BCT BAT ACT AAT.
+
+Definition In_linked_t `{Conc.time BCT} `{Conc.time ACT}
+  (final : BCT) (init : ACT) (t : @link BCT _ ACT _) :=
+  match t with
+  | L bf af =>
+    if leb final bf then
+      eqb final bf = true
+    else
+      eqb init af = true
+  end.
+
+Fixpoint In_linked_ctx `{Conc.time BCT} `{Conc.time ACT}
+  (final : BCT) (init : ACT) (C : @dy_ctx (@link BCT _ ACT _)) :=
+  match C with
+  | [||] => True
+  | dy_c_lam _ t C'
+  | dy_c_lete _ t C' => In_linked_t final init t /\ In_linked_ctx final init C'
+  | dy_c_letm _ C' C'' => In_linked_ctx final init C' /\ In_linked_ctx final init C''
+  end.
+
+Definition In_linked_v `{Conc.time BCT} `{Conc.time ACT}
+  (final : BCT) (init : ACT) (v : @expr_value (@link BCT _ ACT _)) :=
+  match v with
+  | Closure _ _ C => In_linked_ctx final init C
+  end.
+
+Definition In_linked_mem `{Conc.time BCT} `{Conc.time ACT}
+  (final : BCT) (init : ACT) (mem : (@link BCT _ ACT _) -> option (@expr_value (@link BCT _ ACT _))) :=
+  forall t,
+    match mem t with
+    | Some v => In_linked_t final init t /\ In_linked_v final init v
+    | None => True
+    end.
+
+Lemma bound_then_lift_in `{Conc.time BCT} `{Conc.time ACT}
+  (final : BCT) (init : ACT) (C : @dy_ctx BCT) (BOUND : dy_ctx_bound C final) :
+  In_linked_ctx final init (lift_ctx_bf init C).
+Proof.
+  induction C; eauto; destruct BOUND as [BOUND1 BOUND2].
+  - simpl. replace (leb final tx) with false.
+    split; try rewrite eqb_eq; eauto.
+    symmetry. refl_bool. intros contra.
+    assert (final = tx) as RR.
+    apply leb_sym. assumption. apply BOUND1. subst.
+    destruct BOUND1 as [? absurd]. rewrite t_refl in *. inversion absurd.
+  - simpl. replace (leb final tx) with false.
+    split; try rewrite eqb_eq; eauto.
+    symmetry. refl_bool. intros contra.
+    assert (final = tx) as RR.
+    apply leb_sym. assumption. apply BOUND1. subst.
+    destruct BOUND1 as [? absurd]. rewrite t_refl in *. inversion absurd.
+  - simpl. split; eauto.
+Qed.
+
+Definition link_abs `{Conc.time BCT} `{Abs.time BAT} `{Conc.time ACT} `{Abs.time AAT}
+  (final : BCT) (αbf : BCT -> BAT) (αaf : ACT -> AAT) :=
+  fun t =>
+  match t with
+  | L bf af =>
+    if leb final bf then AF (αaf af) else BF (αbf bf)
+  end.
+
+Lemma trans_ctx_lift `{Conc.time BCT} `{Abs.time BAT} `{Conc.time ACT} `{Abs.time AAT}
+  (final : BCT) (init : ACT) (αbf : BCT -> BAT) (αaf : ACT -> AAT) :
+  let αlink := (link_abs final αbf αaf) in
+  forall C (BOUND : dy_ctx_bound C final),
+    trans_ctx αlink (lift_ctx_bf init C) =
+    AL.lift_ctx_bf (trans_ctx αbf C).
+Proof.
+  induction C; simpl; eauto; intros [BOUND1 BOUND2].
+  - replace (leb final tx) with false. rewrite IHC; eauto.
+    symmetry. destruct BOUND1 as [LE NEQ].
+    refl_bool. intros contra. assert (tx = final). apply leb_sym; eauto. subst.
+    rewrite t_refl in NEQ. inversion NEQ.
+  - replace (leb final tx) with false. rewrite IHC; eauto.
+    symmetry. destruct BOUND1 as [LE NEQ].
+    refl_bool. intros contra. assert (tx = final). apply leb_sym; eauto. subst.
+    rewrite t_refl in NEQ. inversion NEQ.
+  - rewrite IHC1; eauto. rewrite IHC2; eauto.
+Qed.
+
+Lemma trans_ctx_filter `{Conc.time BCT} `{Abs.time BAT} `{Conc.time ACT} `{Abs.time AAT}
+  (final : BCT) (init : ACT) (αbf : BCT -> BAT) (αaf : ACT -> AAT) :
+  forall C (INC : In_linked_ctx final init C),
+  let αlink := (link_abs final αbf αaf) in
+  let eqb' t t' := eqb (αlink t) (αlink t') in
+  trans_ctx αaf (CL.filter_ctx_af final C) = AL.filter_ctx_af (trans_ctx αlink C).
+Proof.
+  induction C; simpl; eauto; intros [IN1 IN2].
+  - destruct tx. simpl in *.
+    destruct (leb final bf); simpl; eauto.
+    rewrite IHC; eauto.
+  - destruct tx. simpl in *.
+    destruct (leb final bf); simpl; eauto.
+    rewrite IHC; eauto.
+  - rewrite IHC1; eauto. rewrite IHC2; eauto.
+Qed.
+
+Lemma In_linked_ctx_prefix `{Conc.time BCT} `{Conc.time ACT} eqb
+  (final : BCT) (init : ACT) :
+  forall (Cout C : @dy_ctx (@link BCT _ ACT _))
+         (INC : In_linked_ctx final init C),
+  In_linked_ctx final init (delete_prefix eqb Cout C).
+Proof.
+  induction Cout; intros; eauto.
+  - destruct C; eauto. simpl.
+    destruct (eq_eid x x0) eqn:EQid;
+    destruct (eqb tx tx0) eqn:EQt; eauto.
+    simpl in *. apply IHCout; apply INC.
+  - destruct C; eauto. simpl.
+    destruct (eq_eid x x0) eqn:EQid;
+    destruct (eqb tx tx0) eqn:EQt; eauto.
+    simpl in *. apply IHCout; apply INC.
+  - destruct C; eauto. simpl.
+    destruct (eq_mid M M0) eqn:EQid;
+    destruct (eq_ctx eqb Cout1 C1) eqn:EQC; eauto.
+    simpl in *. apply IHCout2; apply INC.
+Qed.
+
+Lemma In_linked_ctx_map_aux `{Conc.time BCT} `{Conc.time ACT} eqb
+  (final : BCT) (init : ACT) :
+  forall n (C Cout : @dy_ctx (@link BCT _ ACT _)) (LE : dy_level C <= n)
+         (INC : In_linked_ctx final init C),
+  In_linked_ctx final init (delete_map eqb Cout C).
+Proof.
+  induction n; intros; induction C; try reflexivity; try (inversion LE; fail).
+  - rewrite delete_map_red_lam. simpl. simpl in INC.
+    split; try apply INC. apply IHC; try apply INC.
+    simpl in LE. nia.
+  - rewrite delete_map_red_lete. simpl. simpl in INC.
+    split; try apply INC. apply IHC; try apply INC.
+    simpl in LE. nia.
+  - rewrite delete_map_red_letm. simpl. simpl in INC.
+    split. apply IHn. simpl in *.
+    etransitivity. apply delete_prefix_dec. nia.
+    apply In_linked_ctx_prefix. apply INC.
+    apply IHC2. simpl in LE. nia. apply INC.
+Qed.
+
+Lemma In_linked_ctx_delete `{Conc.time BCT} `{Conc.time ACT} eqb
+  (final : BCT) (init : ACT) :
+  forall (Cout C : @dy_ctx (@link BCT _ ACT _))
+         (INC : In_linked_ctx final init C),
+  In_linked_ctx final init (delete_ctx eqb Cout C).
+Proof.
+  intros. unfold delete_ctx.
+  apply In_linked_ctx_map_aux with (n := dy_level C).
+  apply delete_prefix_dec. apply In_linked_ctx_prefix. eauto.
+Qed.
+
+Lemma trans_ctx_link `{Conc.time BCT} `{Abs.time BAT} `{Conc.time ACT} `{Abs.time AAT}
+  (final : BCT) (init : ACT) (Cout : @dy_ctx BCT) (BOUND : dy_ctx_bound Cout final)
+  (αbf : BCT -> BAT) (αaf : ACT -> AAT) :
+  forall C (INC : In_linked_ctx final init C),
+  let αlink := (link_abs final αbf αaf) in
+  let eqb' t t' := eqb (αlink t) (αlink t') in
+  trans_ctx αaf
+    (CL.filter_ctx_af final (delete_ctx eqb' (CL.lift_ctx_bf init Cout) C)) =
+  AL.filter_ctx_af
+    (delete_ctx eqb (AL.lift_ctx_bf (trans_ctx αbf Cout)) (trans_ctx αlink C)).
+Proof.
+  intros.
+  rewrite <- trans_ctx_lift with (final := final) (init := init) (αaf := αaf); eauto.
+  rewrite <- trans_ctx_delete. rewrite trans_ctx_filter with (init := init) (αbf := αbf). eauto.
+  apply In_linked_ctx_delete. eauto.
+Qed.
+
+Lemma In_map_l {T T'} :
+  forall (l : list T) x (f : T -> T'),
+    In x (map f l) <-> exists x', x = f x' /\ In x' l.
+Proof.
+  induction l; simpl; intros.
+  - split; intros contra; try contradict.
+    destruct contra as [x' contra]. apply contra.
+  - split; intros IN.
+    + destruct IN as [L | R].
+      exists a. split; subst; eauto.
+      rewrite IHl in R.
+      destruct R as [x' [EQ IN]].
+      exists x'. eauto.
+    + destruct IN as [x' [EQ [L | R]]].
+      left. subst; eauto.
+      right. rewrite IHl. exists x'. eauto.
+Qed.
+
+Lemma trans_mem_link `{Conc.time BCT} `{Abs.time BAT} `{Conc.time ACT} `{Abs.time AAT}
+  (final : BCT) (init : ACT) (Cout : @dy_ctx BCT) (BOUND : dy_ctx_bound Cout final)
+  (αbf : BCT -> BAT) (αaf : ACT -> AAT) (PRES : preserve_tick αaf) :
+  forall mem abs_mem
+    (EQ : trans_mem (link_abs final αbf αaf) mem abs_mem)
+    (INm : In_linked_mem final init mem),
+  let αlink := (link_abs final αbf αaf) in
+  trans_mem αaf
+  (CL.filter_mem_af final
+     (CL.delete_ctx_mem αlink (CL.lift_ctx_bf init Cout) mem))
+  (AL.filter_mem_af
+     (AL.delete_ctx_mem (AL.lift_ctx_bf (trans_ctx αbf Cout))
+        abs_mem)).
+Proof.
+  intros. subst αlink.
+  red. intros.
+  unfold AL.delete_ctx_mem. unfold AL.filter_mem_af.
+  unfold CL.delete_ctx_mem. unfold CL.filter_mem_af.
+  rewrite In_map_l.
+  split; intros IN.
+  - destruct IN as [v [EQv IN]].
+    rewrite In_map_l in IN.
+    destruct IN as [v' [EQv' IN]].
+    red in EQ. specialize (EQ (AL.AF abs_t) v').
+    rewrite EQ in IN.
+    destruct IN as [t [v'' [TRANSv [TRANSt ACCESS]]]].
+    specialize (INm t). rewrite ACCESS in INm.
+    destruct INm as [INt INv].
+    destruct t. simpl in INt. simpl in TRANSt.
+    destruct (leb final bf); try (inversion TRANSt; fail).
+    rewrite eqb_eq in INt. subst.
+    exists af. rewrite ACCESS.
+    exists (CL.filter_v_af bf
+       (delete_ctx_v
+          (fun t t' : link =>
+           eqb (link_abs bf αbf αaf t)
+             (link_abs bf αbf αaf t'))
+          (CL.lift_ctx_bf init Cout) v'')).
+    repeat split; try (inversion TRANSt; eauto; fail).
+    destruct v''. simpl.
+    rewrite <- trans_ctx_lift with (final := bf) (init := init) (αaf := αaf); eauto.
+    assert (delete_ctx AL.link_eqb
+        (trans_ctx (link_abs bf αbf αaf) (lift_ctx_bf init Cout))
+        (trans_ctx (link_abs bf αbf αaf) C) =
+        trans_ctx (link_abs bf αbf αaf) 
+          (delete_ctx (fun t t' => AL.link_eqb ((link_abs bf αbf αaf) t) ((link_abs bf αbf αaf) t'))
+            (lift_ctx_bf init Cout) C)) as RR.
+    { symmetry. apply (@trans_ctx_delete _ (@AL.link BAT AAT) _ AL.link_eq). }
+    rewrite RR. rewrite trans_ctx_filter with (init := init) (αbf := αbf). eauto.
+    apply In_linked_ctx_delete. eauto.
+  - destruct IN as [af [v [TRANSv [TRANSt SOME]]]].
+    destruct (mem (CL.L final af)) eqn:ACCESS; try (inversion SOME; fail).
+    subst. red in EQ.
+    destruct e. simpl in *.
+    inversion SOME. subst.
+    exists (Closure x e
+      (delete_ctx ALinking.link_eqb
+        (AL.lift_ctx_bf (trans_ctx αbf Cout))
+        (trans_ctx (link_abs final αbf αaf) C))).
+    split. simpl.
+    rewrite <- trans_ctx_lift with (final := final) (init := init) (αaf := αaf); eauto.
+    assert (delete_ctx AL.link_eqb
+        (trans_ctx (link_abs final αbf αaf) (lift_ctx_bf init Cout))
+        (trans_ctx (link_abs final αbf αaf) C) =
+        trans_ctx (link_abs final αbf αaf) 
+          (delete_ctx (fun t t' => AL.link_eqb ((link_abs final αbf αaf) t) ((link_abs final αbf αaf) t'))
+            (lift_ctx_bf init Cout) C)) as RR.
+    { symmetry. apply (@trans_ctx_delete _ (@AL.link BAT AAT) _ AL.link_eq). }
+    rewrite RR. rewrite trans_ctx_filter with (init := init) (αbf := αbf). eauto.
+    apply In_linked_ctx_delete. specialize (INm (CL.L final af)). rewrite ACCESS in INm. apply INm.
+    rewrite In_map_l.
+    exists (Closure x e (trans_ctx (link_abs final αbf αaf) C)).
+    split. eauto.
+    rewrite EQ.
+    exists (CL.L final af).
+    exists (Closure x e C).
+    split; eauto. split; eauto. simpl. rewrite leb_refl. eauto.
+Qed.
+
+Theorem link_abs_pres `{Conc.time BCT} `{Abs.time BAT} `{Conc.time ACT} `{Abs.time AAT}
+  (final : BCT) (init : ACT) (Cout : @dy_ctx BCT) (BOUND : dy_ctx_bound Cout final)
+  (αbf : BCT -> BAT) (αaf : ACT -> AAT) (PRES : preserve_tick αaf) :
+  forall (af : ACT) C mem x v abs_mem
+    (EQ : trans_mem (link_abs final αbf αaf) mem abs_mem)
+    (INm : In_linked_mem final init mem)
+    (INC : In_linked_ctx final init C)
+    (INv : In_linked_v final init v),
+  let αlink := (link_abs final αbf αaf) in
+  αlink (CL.link_tick αlink final init Cout C (ST mem (L final af)) x v) =
+  AL.link_tick (trans_ctx αbf Cout) (trans_ctx αlink C) (Abs.ST abs_mem (AF (αaf af))) x (trans_v αlink v).
+Proof.
+  intros. simpl. rewrite leb_refl. simpl. rewrite leb_refl.
+  assert (αaf
+     (tick
+        (CL.filter_ctx_af final
+           (delete_ctx (fun t t' : CL.link =>
+               ALinking.link_eqb (αlink t) (αlink t'))
+               (CL.lift_ctx_bf init Cout) C))
+        (ST
+           (CL.filter_mem_af final
+              (CL.delete_ctx_mem αlink (CL.lift_ctx_bf init Cout) mem)) af) x
+        (CL.filter_v_af final
+           (delete_ctx_v (fun t t' : CL.link =>
+               ALinking.link_eqb (αlink t) (αlink t'))
+              (CL.lift_ctx_bf init Cout) v))) =
+      Abstract.tick
+     (AL.filter_ctx_af
+        (delete_ctx AL.link_eqb (AL.lift_ctx_bf (trans_ctx αbf Cout))
+           (trans_ctx αlink C)))
+     (Abstract.ST
+        (AL.filter_mem_af
+           (AL.delete_ctx_mem (AL.lift_ctx_bf (trans_ctx αbf Cout))
+              abs_mem)) (αaf af)) x
+     (AL.filter_v_af
+        (delete_ctx_v AL.link_eqb (AL.lift_ctx_bf (trans_ctx αbf Cout))
+           (trans_v αlink v)))) as RR.
+  { 
+    apply PRES. simpl. split. apply trans_ctx_link; eauto.
+    split; try reflexivity. apply trans_mem_link; eauto.
+    destruct v; simpl in *.
+    replace (trans_ctx αaf
+      (CL.filter_ctx_af final
+        (delete_ctx
+           (fun t t' : CL.link =>
+            ALinking.link_eqb (αlink t) (αlink t'))
+           (CL.lift_ctx_bf init Cout) C0))) with
+      (AL.filter_ctx_af
+      (delete_ctx AL.link_eqb (AL.lift_ctx_bf (trans_ctx αbf Cout))
+        (trans_ctx αlink C0))). eauto.
+    symmetry. apply trans_ctx_link; eauto.  
+  }
+  rewrite RR. eauto.
+Qed.
+
